Use λne notation and many clean ups.

F_mu/logrel.v
@@ -12,56 +12,33 @@ Section logrel.
 
   (** Just to get nicer closed forms, we define extend_context_interp in three steps. *)
   Program Definition extend_context_interp_fun1
-    (τi : valC -n> iProp lang Σ)
-    (f : varC -n> valC -n> iProp lang Σ) :
-    (varC -n> valC -n> iProp lang Σ) :=
-    {| cofe_mor_car :=
-         λ x,
-         match x return valC -n> iProp lang Σ with
-         | O => τi
-         | S x' => f x'
-         end
-    |}.
+      (τi : valC -n> iProp lang Σ)
+      (f : varC -n> valC -n> iProp lang Σ) :
+      (varC -n> valC -n> iProp lang Σ) := λne x,
+    match x return valC -n> iProp lang Σ with O => τi | S x' => f x' end.
 
   Program Definition extend_context_interp_fun2
     (τi : valC -n> iProp lang Σ) :
     (varC -n> valC -n> iProp lang Σ) -n>
-    (varC -n> valC -n> iProp lang Σ) :=
-    {|
-      cofe_mor_car := λ f, extend_context_interp_fun1 τi f
-    |}.
-  Next Obligation.
-  Proof. intros ???? Hfg x; destruct x; cbn; trivial. Qed.
+    (varC -n> valC -n> iProp lang Σ) := λne f, extend_context_interp_fun1 τi f.
+  Next Obligation. intros ???? Hfg x; destruct x; cbn; trivial. Qed.
 
   Program Definition extend_context_interp :
     (valC -n> iProp lang Σ) -n>
     (varC -n> valC -n> iProp lang Σ) -n>
-    (varC -n> valC -n> iProp lang Σ) :=
-    {|
-      cofe_mor_car := λ τi, extend_context_interp_fun2 τi
-    |}.
-  Next Obligation.
-  Proof. intros n g h H Δ x y. destruct x; cbn; auto. Qed.
+    (varC -n> valC -n> iProp lang Σ) := λne τi, extend_context_interp_fun2 τi.
+  Next Obligation. intros n g h H Δ x y. destruct x; cbn; auto. Qed.
 
   Program Definition extend_context_interp_apply :
-    ((varC -n> valC -n> iProp lang Σ)) -n>
-    ((varC -n> valC -n> iProp lang Σ) -n>
-     valC -n> iProp lang Σ) -n>
-    (valC -n> iProp lang Σ) -n> (valC -n> iProp lang Σ) :=
-    {|
-      cofe_mor_car := λ Δ,
-        {|
-          cofe_mor_car := λ f,
-            {|
-              cofe_mor_car := λ g, f (extend_context_interp g Δ)
-            |}
-        |}
-    |}.
+      ((varC -n> valC -n> iProp lang Σ)) -n>
+      ((varC -n> valC -n> iProp lang Σ) -n>
+       valC -n> iProp lang Σ) -n>
+      (valC -n> iProp lang Σ) -n> (valC -n> iProp lang Σ) := λne Δ f g,
+    f (extend_context_interp g Δ).
   Solve Obligations with
   repeat intros ?; (cbn + idtac);
     try match goal with [H : _ ≡{_}≡ _|- _] => rewrite H end; trivial.
   Next Obligation.
-  Proof.
     intros n Δ Δ' HΔ f g x.  cbn.
     match goal with
       |- _ _ ?F x ≡{n}≡ _ _ ?G x =>
@@ -71,173 +48,71 @@ Section logrel.
     destruct y; trivial.
   Qed.
 
-  Definition interp_unit : valC -n> iProp lang Σ :=
-    {|
-      cofe_mor_car := λ w, (w = UnitV)%I
-    |}.
+  Definition interp_unit : valC -n> iProp lang Σ := λne w, (w = UnitV)%I.
 
   Program Definition interp_prod :
-    (valC -n> iProp lang Σ) -n> (valC -n> iProp lang Σ) -n>
-    valC -n> iProp lang Σ :=
-    {|
-      cofe_mor_car :=
-        λ τ1i,
-        {|
-          cofe_mor_car :=
-            λ τ2i,
-            {|
-              cofe_mor_car :=
-                λ w, (∃ w1 w2, w = PairV w1 w2 ∧ τ1i w1 ∧ τ2i w2)%I
-            |}
-        |}
-    |}.
-  Solve Obligations with
-  repeat intros ?; cbn;
-    repeat apply exist_ne =>?;
-        try match goal with [H : _ ≡{_}≡ _|- _] => rewrite H end; trivial.
+      (valC -n> iProp lang Σ) -n> (valC -n> iProp lang Σ) -n>
+      valC -n> iProp lang Σ := λne τ1i τ2i w,
+    (∃ w1 w2, w = PairV w1 w2 ∧ τ1i w1 ∧ τ2i w2)%I.
+  Solve Obligations with solve_proper.
 
   Program Definition interp_sum :
-    (valC -n> iProp lang Σ) -n> (valC -n> iProp lang Σ) -n>
-    valC -n> iProp lang Σ :=
-    {|
-      cofe_mor_car :=
-        λ τ1i,
-        {|
-          cofe_mor_car :=
-            λ τ2i,
-            {|
-              cofe_mor_car :=
-                λ w, ((∃ w1, w = InjLV w1 ∧ τ1i w1) ∨
-                      (∃ w2, w = InjRV w2 ∧ τ2i w2))%I
-            |}
-        |}
-    |}.
-  Solve Obligations with
-  repeat intros ?; cbn; try apply or_ne;
-    try apply exist_ne =>?;
-        try match goal with [H : _ ≡{_}≡ _|- _] => rewrite H end; trivial.
+      (valC -n> iProp lang Σ) -n> (valC -n> iProp lang Σ) -n>
+      valC -n> iProp lang Σ := λne τ1i τ2i w,
+    ((∃ w1, w = InjLV w1 ∧ τ1i w1) ∨ (∃ w2, w = InjRV w2 ∧ τ2i w2))%I.
+  Solve Obligations with solve_proper.
 
   Program Definition interp_arrow :
-    (valC -n> iProp lang Σ) -n> (valC -n> iProp lang Σ) -n>
-    valC -n> iProp lang Σ :=
-    {|
-      cofe_mor_car :=
-        λ τ1i,
-        {|
-          cofe_mor_car :=
-            λ τ2i,
-            {|
-              cofe_mor_car :=
-                λ w, (□ ∀ v, τ1i v → WP App (# w) (# v) {{τ2i}})%I
-            |}
-        |}
-    |}.
-  Solve Obligations with
-  repeat intros ?; cbn;
-    try apply always_ne;
-    try apply forall_ne=>?; try apply impl_ne; trivial;
-      try apply wp_ne =>?;
-          try match goal with [H : _ ≡{_}≡ _|- _] => rewrite H end; trivial.
+      (valC -n> iProp lang Σ) -n> (valC -n> iProp lang Σ) -n>
+      valC -n> iProp lang Σ := λne τ1i τ2i w,
+    (□ ∀ v, τ1i v → WP App (# w) (# v) {{ τ2i }})%I.
+  Solve Obligations with solve_proper.
 
   Program Definition interp_forall :
-    ((valC -n> iProp lang Σ) -n> (valC -n> iProp lang Σ)) -n>
-    valC -n> iProp lang Σ :=
-    {|
-      cofe_mor_car :=
-        λ τi,
-        {|
-          cofe_mor_car :=
-            λ w,
-            (∀ (τ'i : {f : (valC -n> iProp lang Σ) | ∀ v, PersistentP (f v)}%type),
-                □ WP TApp (# w) {{λ v, (τi (`τ'i) v)}})%I
-        |}
-    |}.
-  Next Obligation.
-  Proof.
-    intros τ τ' x y Hxy; cbn; rewrite Hxy; trivial.
-  Qed.
-  Next Obligation.
-    intros n f g Hfg x; cbn.
-    apply forall_ne=> P.
-    apply always_ne, wp_ne => w.
-    rewrite Hfg; trivial.
-  Qed.
+      ((valC -n> iProp lang Σ) -n> (valC -n> iProp lang Σ)) -n>
+      valC -n> iProp lang Σ := λne τi w,
+    (∀ τ'i : valC -n> iProp lang Σ,
+      □ (■ (∀ v, PersistentP (τ'i v)) → WP TApp (# w) {{ τi τ'i }}))%I.
+  Solve Obligations with solve_proper.
 
   Program Definition interp_rec_pre :
-    ((valC -n> iProp lang Σ) -n> (valC -n> iProp lang Σ)) -n>
-    (valC -n> iProp lang Σ) -n>
-    (valC -n> iProp lang Σ) :=
-    {|
-      cofe_mor_car :=
-        λ τi,
-        {| cofe_mor_car :=
-             λ rec_appr,
-             {|
-               cofe_mor_car := λ w, (□ (∃ v, w = FoldV v ∧ ▷ (τi rec_appr v)))%I
-             |}
-        |}
-    |}.
-  Next Obligation.
-  Proof.
-    intros τi rec_appr n x y Hxy; rewrite Hxy; trivial.
-  Qed.
-  Next Obligation.
-  Proof.
-    intros τi n f g Hfg x. cbn.
-    apply always_ne, exist_ne =>w; rewrite Hfg; trivial.
-  Qed.
-  Next Obligation.
-  Proof.
-    intros n τi τi' Hτi f x. cbn.
-    apply always_ne, exist_ne =>w; rewrite Hτi; trivial.
-  Qed.
+      ((valC -n> iProp lang Σ) -n> (valC -n> iProp lang Σ)) -n>
+      (valC -n> iProp lang Σ) -n>
+      (valC -n> iProp lang Σ) := λne τi rec_appr w,
+    (□ (∃ v, w = FoldV v ∧ ▷ τi rec_appr v))%I.
+  Solve Obligations with solve_proper.
 
   Global Instance interp_rec_pre_contr
-           (τi : (valC -n> iProp lang Σ) -n> (valC -n> iProp lang Σ))
-    :
-      Contractive (interp_rec_pre τi).
+      (τi : (valC -n> iProp lang Σ) -n> (valC -n> iProp lang Σ)) :
+    Contractive (interp_rec_pre τi).
   Proof.
     intros n f g H w; cbn.
     apply always_ne, exist_ne; intros e; apply and_ne; trivial.
-    apply later_contractive =>i Hi.
-    rewrite H; trivial.
+    apply later_contractive =>i Hi. rewrite H; trivial.
   Qed.
 
   Program Definition interp_rec :
     ((valC -n> iProp lang Σ) -n> (valC -n> iProp lang Σ)) -n>
-    (valC -n> iProp lang Σ)
-    :=
-      {|
-        cofe_mor_car := λ τi, fixpoint (interp_rec_pre τi)
-      |}.
-  Next Obligation.
-  Proof. intros n f g H; apply fixpoint_ne => z; rewrite H; trivial. Qed.
+    (valC -n> iProp lang Σ) := λne τi, fixpoint (interp_rec_pre τi).
+  Next Obligation. intros n f g H; apply fixpoint_ne => z; rewrite H; trivial. Qed.
 
-  Program Fixpoint interp (τ : type) {struct τ}
-    : (varC -n> (valC -n> iProp lang Σ)) -n> valC -n> iProp lang Σ
-    :=
-      match τ with
-        | TUnit => {| cofe_mor_car := λ Δ, interp_unit |}
-        | TProd τ1 τ2 =>
-          {| cofe_mor_car := λ Δ, interp_prod (interp τ1 Δ) (interp τ2 Δ)|}
-        | TSum τ1 τ2 => {| cofe_mor_car := λ Δ,interp_sum (interp τ1 Δ) (interp τ2 Δ)|}
-        | TArrow τ1 τ2 => {|cofe_mor_car := λ Δ, interp_arrow (interp τ1 Δ) (interp τ2 Δ)|}
-        | TVar v => {| cofe_mor_car :=
-                        λ Δ : (varC -n> (valC -n> iProp lang Σ)), (Δ v) |}
-        | TForall τ' =>
-          {| cofe_mor_car := λ Δ,
-                             interp_forall (extend_context_interp_apply Δ (interp τ'))|}
-        | TRec τ' =>
-          {| cofe_mor_car := λ Δ,
-                             interp_rec (extend_context_interp_apply Δ (interp τ'))|}
-        end%I.
+  Program Fixpoint interp (τ : type) {struct τ} :
+      (varC -n> (valC -n> iProp lang Σ)) -n> valC -n> iProp lang Σ :=
+    match τ with
+    | TUnit => λne Δ, interp_unit
+    | TProd τ1 τ2 => λne Δ, interp_prod (interp τ1 Δ) (interp τ2 Δ)
+    | TSum τ1 τ2 => λne Δ, interp_sum (interp τ1 Δ) (interp τ2 Δ)
+    | TArrow τ1 τ2 => λne Δ, interp_arrow (interp τ1 Δ) (interp τ2 Δ)
+    | TVar v => λne Δ : varC -n> (valC -n> iProp lang Σ), (Δ v)
+    | TForall τ' => λne Δ, interp_forall (extend_context_interp_apply Δ (interp τ'))
+    | TRec τ' => λne Δ, interp_rec (extend_context_interp_apply Δ (interp τ'))
+    end%I.
   Solve Obligations with
   repeat intros ?; match goal with [H : _ ≡{_}≡ _|- _] => rewrite H end; trivial.
 
   Global Instance interp_Persistent
-         τ (Δ : varC -n> valC -n> iProp lang Σ)
-         {HΔ : ∀ x v, PersistentP (Δ x v)}
-    : ∀ v, PersistentP (interp τ Δ v).
+      τ (Δ : varC -n> valC -n> iProp lang Σ) {HΔ : ∀ x v, PersistentP (Δ x v)} :
+    ∀ v, PersistentP (interp τ Δ v).
   Proof.
     revert Δ HΔ.
     induction τ; cbn; intros Δ HΔ v; try apply _.
@@ -246,33 +121,31 @@ Section logrel.
   Qed.
 
   Global Instance extend_context_interp_Persistent
-    (f : valC -n> iProp lang Σ) (Δ : varC -n> valC -n> iProp lang Σ)
-           (Hf : ∀ v, PersistentP (f v))
-           {HΔ : ∀ x v, PersistentP (Δ x v)}
-    : ∀ x v, PersistentP (@extend_context_interp f Δ x v).
+      (f : valC -n> iProp lang Σ) (Δ : varC -n> valC -n> iProp lang Σ)
+      (Hf : ∀ v, PersistentP (f v))
+      {HΔ : ∀ x v, PersistentP (Δ x v)} :
+    ∀ x v, PersistentP (@extend_context_interp f Δ x v).
   Proof. intros x v. destruct x; cbn; trivial. Qed.
 
   Local Ltac properness :=
     repeat
-      match goal with
-      | |- (∃ _: _, _)%I ≡ (∃ _: _, _)%I => apply exist_proper =>?
-      | |- (∀ _: _, _)%I ≡ (∀ _: _, _)%I => apply forall_proper =>?
-      | |- (_ ∧ _)%I ≡ (_ ∧ _)%I => apply and_proper
-      | |- (_ ∨ _)%I ≡ (_ ∨ _)%I => apply or_proper
-      | |- (_ → _)%I ≡ (_ → _)%I => apply impl_proper
-      | |- (WP _ {{ _ }})%I ≡ (WP _ {{ _ }})%I => apply wp_proper =>?
-      | |- (▷ _)%I ≡ (▷ _)%I => apply later_proper
-      | |- (□ _)%I ≡ (□ _)%I => apply always_proper
-      end.
+    match goal with
+    | |- (∃ _: _, _)%I ≡ (∃ _: _, _)%I => apply exist_proper =>?
+    | |- (∀ _: _, _)%I ≡ (∀ _: _, _)%I => apply forall_proper =>?
+    | |- (_ ∧ _)%I ≡ (_ ∧ _)%I => apply and_proper
+    | |- (_ ∨ _)%I ≡ (_ ∨ _)%I => apply or_proper
+    | |- (_ → _)%I ≡ (_ → _)%I => apply impl_proper
+    | |- (WP _ {{ _ }})%I ≡ (WP _ {{ _ }})%I => apply wp_proper =>?
+    | |- (▷ _)%I ≡ (▷ _)%I => apply later_proper
+    | |- (□ _)%I ≡ (□ _)%I => apply always_proper
+    end.
 
   Lemma interp_unused_contex_irrel
-        (m n : nat)
-        (Δ Δ' : varC -n> valC -n> iProp lang Σ)
-        (HΔ : ∀ v, Δ (if lt_dec v m then v else (n + v)) ≡
-                     Δ' (if lt_dec v m then v else (n + v)))
-        (τ : type)
-    :
-      interp τ.[iter m up (ren (+n))] Δ ≡ interp τ.[iter m up (ren (+n))] Δ'.
+      (m n : nat) (Δ Δ' : varC -n> valC -n> iProp lang Σ)
+      (HΔ : ∀ v, Δ (if lt_dec v m then v else (n + v)) ≡
+                   Δ' (if lt_dec v m then v else (n + v)))
+      (τ : type) :
+    interp τ.[iter m up (ren (+n))] Δ ≡ interp τ.[iter m up (ren (+n))] Δ'.
   Proof.
     revert m n Δ Δ' HΔ.
     induction τ; intros m n Δ Δ' HΔ v; cbn; auto.
@@ -314,28 +187,21 @@ Section logrel.
   Qed.
 
   Program Definition hop_context_interp (m n : nat) :
-    (varC -n> valC -n> iProp lang Σ) -n>
-    (varC -n> valC -n> iProp lang Σ) :=
-    {| cofe_mor_car :=
-         λ Δ,
-         {| cofe_mor_car := λ v, if lt_dec v m then Δ v else Δ (v - n) |}
-    |}.
+      (varC -n> valC -n> iProp lang Σ) -n>
+      (varC -n> valC -n> iProp lang Σ) := λne Δ v,
+    if lt_dec v m then Δ v else Δ (v - n).
+  Next Obligation. intros ?????? Hxy; destruct Hxy; trivial. Qed.
   Next Obligation.
-  Proof. intros ?????? Hxy; destruct Hxy; trivial. Qed.
-  Next Obligation.
-  Proof.
     intros ????? Hfg ?; cbn. destruct lt_dec; rewrite Hfg; trivial.
   Qed.
 
   Lemma extend_bofore_hop_context_interp (m n : nat)
-        (Δ : varC -n> valC -n> iProp lang Σ)
-        (τi : valC -n> iProp lang Σ)
-        (v : var)
-    :
-      (extend_context_interp τi (hop_context_interp m n Δ)
-                             (if lt_dec v (S m) then v else n + v))
-        ≡ (hop_context_interp (S m) n (extend_context_interp τi Δ)
-                              (if lt_dec v (S m) then v else n + v)).
+      (Δ : varC -n> valC -n> iProp lang Σ)
+      (τi : valC -n> iProp lang Σ) (v : var) :
+    (extend_context_interp τi (hop_context_interp m n Δ)
+                              (if lt_dec v (S m) then v else n + v))
+    ≡ (hop_context_interp (S m) n (extend_context_interp τi Δ)
+                                  (if lt_dec v (S m) then v else n + v)).
   Proof.
     destruct v; cbn; trivial.
     repeat (destruct lt_dec; cbn); auto with omega.
@@ -347,10 +213,8 @@ Section logrel.
   Qed.
 
   Lemma interp_subst_weaken
-        (m n : nat)
-        (Δ : varC -n> valC -n> iProp lang Σ)
-        (τ : type)
-    : interp τ Δ ≡ interp τ.[iter m up (ren (+n))] (hop_context_interp m n Δ).
+      (m n : nat) (Δ : varC -n> valC -n> iProp lang Σ) (τ : type) :
+    interp τ Δ ≡ interp τ.[iter m up (ren (+n))] (hop_context_interp m n Δ).
   Proof.
     revert m n Δ.
     induction τ; intros m n Δ v; cbn -[extend_context_interp]; auto.
@@ -371,12 +235,7 @@ Section logrel.
       asimpl; unfold ids; cbn; destruct lt_dec; cbn; destruct lt_dec; auto with omega.
       replace (m + n + (x - m)) with (x + n) by omega.
       replace (x + n - n) with x; trivial.
-      { (** An incompleteness in omega and lia! *)
-        clear.
-        replace (x + n) with (n + x) by omega.
-        induction n; cbn; auto with omega.
-        induction x; cbn; trivial.
-      }
+      { unfold var in *; omega. }
     - properness; trivial.
       change (up (iter m up (ren (+n)))) with (iter (S m) up (ren (+n))).
       rewrite IHτ.
@@ -385,9 +244,9 @@ Section logrel.
   Qed.
 
   Lemma interp_ren_S (τ : type)
-        (Δ : varC -n> valC -n> iProp lang Σ)
-        (τi : valC -n> iProp lang Σ)
-    : interp τ Δ ≡ interp τ.[ren (+1)] (extend_context_interp τi Δ).
+      (Δ : varC -n> valC -n> iProp lang Σ)
+      (τi : valC -n> iProp lang Σ) :
+    interp τ Δ ≡ interp τ.[ren (+1)] (extend_context_interp τi Δ).
   Proof.
     rewrite (interp_subst_weaken 0 1).
     apply interp_unused_contex_irrel.
@@ -399,37 +258,24 @@ Section logrel.
   Program Definition context_interp_insert (m : nat) :
     (valC -n> iProp lang Σ) -n>
     (varC -n> valC -n> iProp lang Σ) -n>
-    (varC -n> valC -n> iProp lang Σ) :=
-    {| cofe_mor_car :=
-         λ τi,
-         {| cofe_mor_car :=
-              λ Δ,
-              {| cofe_mor_car :=
-                   λ v, if lt_dec v m then Δ v else
-                          if eq_nat_dec v m then τi else Δ (v - 1)
-              |}
-         |}
-    |}.
+    (varC -n> valC -n> iProp lang Σ) := λne τi Δ v,
+      if lt_dec v m then Δ v else if eq_nat_dec v m then τi else Δ (v - 1).
+  Next Obligation. intros m τi Δ n x y Hxy; destruct Hxy; trivial. Qed.
   Next Obligation.
-  Proof. intros m τi Δ n x y Hxy; destruct Hxy; trivial. Qed.
-  Next Obligation.
-  Proof.
     intros m τi n Δ Δ' HΔ x; cbn;
       destruct lt_dec; try destruct eq_nat_dec; auto.
   Qed.
   Next Obligation.
-  Proof.
     intros m n f g Hfg F Δ x; cbn;
       destruct lt_dec; try destruct eq_nat_dec; auto.
   Qed.
 
   Lemma extend_context_interp_insert (m : nat)
-        (τi : valC -n> iProp lang Σ)
-        (Δ : varC -n> valC -n> iProp lang Σ)
-        (Ti : valC -n> iProp lang Σ)
-    :
-      (extend_context_interp Ti (context_interp_insert m τi Δ))
-        ≡ (context_interp_insert (S m) τi (extend_context_interp Ti Δ)).
+      (τi : valC -n> iProp lang Σ)
+      (Δ : varC -n> valC -n> iProp lang Σ)
+      (Ti : valC -n> iProp lang Σ) :
+    extend_context_interp Ti (context_interp_insert m τi Δ)
+    ≡ context_interp_insert (S m) τi (extend_context_interp Ti Δ).
   Proof.
     intros [|v]; cbn; trivial.
     repeat destruct lt_dec; trivial;
@@ -439,11 +285,8 @@ Section logrel.
   Qed.
 
   Lemma context_interp_insert_O_extend
-        (τi : valC -n> iProp lang Σ)
-        (Δ : varC -n> valC -n> iProp lang Σ)
-    :
-      (context_interp_insert O τi Δ)
-        ≡ (extend_context_interp τi Δ).
+      (τi : valC -n> iProp lang Σ) (Δ : varC -n> valC -n> iProp lang Σ) :
+    context_interp_insert O τi Δ ≡ extend_context_interp τi Δ.
   Proof.
     intros [|v]; cbn; trivial.
     repeat destruct lt_dec; trivial;
@@ -451,9 +294,8 @@ Section logrel.
     destruct v; cbn; auto with omega.
   Qed.
 
-  Lemma iter_up_subst_type (m : nat) (τ : type) (x : var)
-    :
-      (iter m up (τ .: ids) x) =
+  Lemma iter_up_subst_type (m : nat) (τ : type) (x : var) :
+    iter m up (τ .: ids) x =
       if lt_dec x m then ids x else
         if eq_nat_dec x m then τ.[ren (+m)] else ids (x - 1).
   Proof.
@@ -470,12 +312,11 @@ Section logrel.
   Qed.
 
   Lemma interp_subst_iter_up
-        (m : nat)
-        (Δ : varC -n> valC -n> iProp lang Σ)
-        (τ : type)
-        (τ' : type)
-    : interp τ (context_interp_insert m (interp τ'.[ren (+m)] Δ) Δ)
-             ≡ interp τ.[iter m up (τ' .: ids)] Δ.
+      (m : nat)
+      (Δ : varC -n> valC -n> iProp lang Σ)
+      (τ : type) (τ' : type) :
+    interp τ (context_interp_insert m (interp τ'.[ren (+m)] Δ) Δ)
+    ≡ interp τ.[iter m up (τ' .: ids)] Δ.
   Proof.
     revert m Δ.
     induction τ; intros m Δ v; cbn -[extend_context_interp]; auto.
@@ -505,10 +346,9 @@ Section logrel.
   Qed.
 
   Lemma interp_subst
-        (Δ : varC -n> valC -n> iProp lang Σ)
-        (τ : type)
-        (τ' : type)
-    : interp τ (extend_context_interp (interp τ' Δ) Δ) ≡ interp τ.[τ'/] Δ.
+      (Δ : varC -n> valC -n> iProp lang Σ)
+      (τ : type) (τ' : type) :
+    interp τ (extend_context_interp (interp τ' Δ) Δ) ≡ interp τ.[τ'/] Δ.
   Proof.
     rewrite -(interp_subst_iter_up O Δ τ τ').
     rewrite context_interp_insert_O_extend.
@@ -518,15 +358,13 @@ Section logrel.
   Lemma zip_with_context_interp_subst
         (Δ : varC -n> valC -n> iProp lang Σ) (Γ : list type)
         (vs : list valC) (τi : valC -n> iProp lang Σ) :
-    (([∧] zip_with (λ τ, interp τ Δ) Γ vs)%I)
-      ≡ ([∧] zip_with (λ τ, interp τ (extend_context_interp τi Δ))
-                    (map (λ t : type, t.[ren (+1)]) Γ) vs)%I.
+    ([∧] zip_with (λ τ, interp τ Δ) Γ vs)
+    ⊣⊢ ([∧] zip_with (λ τ, interp τ (extend_context_interp τi Δ))
+                    (map (λ t : type, t.[ren (+1)]) Γ) vs).
   Proof.
     revert Δ vs τi.
     induction Γ as [|Γ]; intros Δ vs τi; cbn; trivial.
     destruct vs; cbn; trivial.
-    apply and_proper.
-    - apply interp_ren_S.
-    - apply IHΓ.
+    apply and_proper. apply interp_ren_S. apply IHΓ.
   Qed.
 End logrel.
