F_mu_ref_par/logrel_binary.v
@@ -20,56 +20,35 @@ Section logrel.
   (** Just to get nicer closed forms, we define extend_context_interp in
       three steps. *)
   Program Definition extend_context_interp_fun1
-    (τi : bivalC -n> iPropG lang Σ)
-    (f : varC -n> bivalC -n> iPropG lang Σ) :
-    (varC -n> bivalC -n> iPropG lang Σ) :=
-    {| cofe_mor_car :=
-         λ x,
-         match x return bivalC -n> iPropG lang Σ with
-         | O => τi
-         | S x' => f x'
-         end
-    |}.
+      (τi : bivalC -n> iPropG lang Σ)
+      (f : varC -n> bivalC -n> iPropG lang Σ) :
+      (varC -n> bivalC -n> iPropG lang Σ) := λne x,
+    match x return bivalC -n> iPropG lang Σ with O => τi | S x' => f x' end.
 
   Program Definition extend_context_interp_fun2
-    (τi : bivalC -n> iPropG lang Σ) :
-    (varC -n> bivalC -n> iPropG lang Σ) -n>
-    (varC -n> bivalC -n> iPropG lang Σ) :=
-    {|
-      cofe_mor_car := λ f, extend_context_interp_fun1 τi f
-    |}.
-  Next Obligation.
-  Proof. intros ???? Hfg x; destruct x; cbn; trivial. Qed.
+      (τi : bivalC -n> iPropG lang Σ) :
+      (varC -n> bivalC -n> iPropG lang Σ) -n>
+      (varC -n> bivalC -n> iPropG lang Σ) := λne f,
+    extend_context_interp_fun1 τi f.
+  Next Obligation. intros ???? Hfg x; destruct x; cbn; trivial. Qed.
 
   Program Definition extend_context_interp :
-    (bivalC -n> iPropG lang Σ) -n>
-    (varC -n> bivalC -n> iPropG lang Σ) -n>
-    (varC -n> bivalC -n> iPropG lang Σ) :=
-    {|
-      cofe_mor_car := λ τi, extend_context_interp_fun2 τi
-    |}.
-  Next Obligation.
-  Proof. intros n g h H Δ x y. destruct x; cbn; auto. Qed.
+      (bivalC -n> iPropG lang Σ) -n>
+      (varC -n> bivalC -n> iPropG lang Σ) -n>
+      (varC -n> bivalC -n> iPropG lang Σ) := λne τi,
+    extend_context_interp_fun2 τi.
+  Next Obligation. intros n g h H Δ x y. destruct x; cbn; auto. Qed.
 
   Program Definition extend_context_interp_apply :
-    ((varC -n> bivalC -n> iPropG lang Σ)) -n>
-    ((varC -n> bivalC -n> iPropG lang Σ) -n>
-     bivalC -n> iPropG lang Σ) -n>
-    (bivalC -n> iPropG lang Σ) -n> (bivalC -n> iPropG lang Σ) :=
-    {|
-      cofe_mor_car := λ Δ,
-        {|
-          cofe_mor_car := λ f,
-            {|
-              cofe_mor_car := λ g, f (extend_context_interp g Δ)
-            |}
-        |}
-    |}.
+      ((varC -n> bivalC -n> iPropG lang Σ)) -n>
+      ((varC -n> bivalC -n> iPropG lang Σ) -n>
+       bivalC -n> iPropG lang Σ) -n>
+      (bivalC -n> iPropG lang Σ) -n> (bivalC -n> iPropG lang Σ) := λne Δ f g,
+    f (extend_context_interp g Δ).
   Solve Obligations with
   repeat intros ?; (cbn + idtac);
     try match goal with [H : _ ≡{_}≡ _|- _] => rewrite H end; trivial.
   Next Obligation.
-  Proof.
     intros n Δ Δ' HΔ f g x.  cbn.
     match goal with
       |- _ _ ?F x ≡{n}≡ _ _ ?G x =>
@@ -79,274 +58,136 @@ Section logrel.
     destruct y; trivial.
   Qed.
 
-  Program Definition interp_unit : bivalC -n> iPropG lang Σ :=
-    {|
-      cofe_mor_car := λ w, (w.1 = UnitV ∧ w.2 = UnitV)%I
-    |}.
-  Next Obligation.
-  Proof. intros n x y [H1 H2]; rewrite H1 H2; trivial. Qed.
+  Program Definition interp_unit : bivalC -n> iPropG lang Σ := λne w,
+    (w.1 = UnitV ∧ w.2 = UnitV)%I.
+  Next Obligation. intros n x y [H1 H2]; rewrite H1 H2; trivial. Qed.
 
-  Program Definition interp_nat : bivalC -n> iPropG lang Σ :=
-    {|
-      cofe_mor_car := λ w, (∃ n, w.1 = (♯v n) ∧ w.2 = (♯v n))%I
-    |}.
-  Next Obligation.
-  Proof. intros n x y [H1 H2]; rewrite H1 H2; trivial. Qed.
+  Program Definition interp_nat : bivalC -n> iPropG lang Σ := λne w,
+    (∃ n, w.1 = (♯v n) ∧ w.2 = (♯v n))%I.
+  Next Obligation. intros n x y [H1 H2]; rewrite H1 H2; trivial. Qed.
 
-  Program Definition interp_bool : bivalC -n> iPropG lang Σ :=
-    {|
-      cofe_mor_car := λ w, (∃ b, w.1 = (♭v b) ∧ w.2 = (♭v b))%I
-    |}.
-  Next Obligation.
-  Proof. intros n x y [H1 H2]; rewrite H1 H2; trivial. Qed.
+  Program Definition interp_bool : bivalC -n> iPropG lang Σ :=λne w,
+    (∃ b, w.1 = (♭v b) ∧ w.2 = (♭v b))%I.
+  Next Obligation. intros n x y [H1 H2]; rewrite H1 H2; trivial. Qed.
 
   Program Definition interp_prod :
-    (bivalC -n> iPropG lang Σ) -n> (bivalC -n> iPropG lang Σ) -n>
-    bivalC -n> iPropG lang Σ :=
-    {|
-      cofe_mor_car :=
-        λ τ1i,
-        {|
-          cofe_mor_car :=
-            λ τ2i,
-            {|
-              cofe_mor_car :=
-                λ w, (∃ w1 w2, w = (PairV (w1.1) (w1.2), PairV (w2.1) (w2.2)) ∧
-                               τ1i (w1.1, w2.1) ∧ τ2i (w1.2, w2.2))%I
-            |}
-        |}
-    |}.
+      (bivalC -n> iPropG lang Σ) -n> (bivalC -n> iPropG lang Σ) -n>
+      bivalC -n> iPropG lang Σ := λne τ1i τ2i w,
+    (∃ w1 w2, w = (PairV (w1.1) (w1.2), PairV (w2.1) (w2.2)) ∧
+              τ1i (w1.1, w2.1) ∧ τ2i (w1.2, w2.2))%I.
   Next Obligation.
-  Proof.
     intros τ1i τ2i n [x1 x2] [y1 y2] [H1 H2]; simpl in *.
     rewrite H1 H2; trivial.
   Qed.
-  Next Obligation.
-  Proof.
-    intros τ1i n τi τi' Hτi y; simpl.
-    apply exist_ne => z; apply exist_ne => z'.
-    rewrite Hτi; trivial.
-  Qed.
-  Next Obligation.
-    intros n τi τi' Hτi τ2i y; simpl.
-    apply exist_ne => z; apply exist_ne => z'.
-    rewrite Hτi; trivial.
-  Qed.
+  Next Obligation. solve_proper. Qed.
+  Next Obligation. solve_proper. Qed.
 
   Program Definition interp_sum :
-    (bivalC -n> iPropG lang Σ) -n> (bivalC -n> iPropG lang Σ) -n>
-    bivalC -n> iPropG lang Σ :=
-    {|
-      cofe_mor_car :=
-        λ τ1i,
-        {|
-          cofe_mor_car :=
-            λ τ2i,
-            {|
-              cofe_mor_car :=
-                λ w, ((∃ w1, w = (InjLV (w1.1), InjLV (w1.2)) ∧ τ1i w1) ∨
-                      (∃ w2, w = (InjRV (w2.1), InjRV (w2.2)) ∧ τ2i w2))%I
-            |}
-        |}
-    |}.
+      (bivalC -n> iPropG lang Σ) -n> (bivalC -n> iPropG lang Σ) -n>
+      bivalC -n> iPropG lang Σ := λne τ1i τ2i w,
+    ((∃ w1, w = (InjLV (w1.1), InjLV (w1.2)) ∧ τ1i w1) ∨
+     (∃ w2, w = (InjRV (w2.1), InjRV (w2.2)) ∧ τ2i w2))%I.
   Next Obligation.
-  Proof.
     intros τ1i τ2i n [x1 x2] [y1 y2] [H1 H2]; simpl in *.
     rewrite H1 H2; trivial.
   Qed.
-  Next Obligation.
-  Proof.
-    intros τ1i n τi τi' Hτi y; simpl.
-    apply or_ne; apply exist_ne => z; trivial.
-    rewrite Hτi; trivial.
-  Qed.
-  Next Obligation.
-    intros n τi τi' Hτi τ2i y; simpl.
-    apply or_ne; apply exist_ne => z; trivial.
-    rewrite Hτi; trivial.
-  Qed.
+  Next Obligation. solve_proper. Qed.
+  Next Obligation. solve_proper. Qed.
 
   Context `{Si : cfgSG Σ}.
 
   Program Definition interp_arrow :
-    (bivalC -n> iPropG lang Σ) -n> (bivalC -n> iPropG lang Σ) -n>
-    bivalC -n> iPropG lang Σ :=
-    {|
-      cofe_mor_car :=
-        λ τ1i,
-        {|
-          cofe_mor_car :=
-            λ τ2i,
-            {|
-              cofe_mor_car :=
-                λ w, (□ ∀ j K v,
-                           τ1i v ★ j ⤇ (fill K (App (# w.2) (# v.2))) →
-                           WP App (# w.1) (# v.1)
-                              {{z, ∃ z', j ⤇ (fill K (# z')) ★ τ2i (z, z')}})%I
-            |}
-        |}
-    |}.
-  Next Obligation.
+      (bivalC -n> iPropG lang Σ) -n> (bivalC -n> iPropG lang Σ) -n>
+      bivalC -n> iPropG lang Σ := λne τ1i τ2i w,
+    (□ ∀ j K v,
+      τ1i v ★ j ⤇ (fill K (App (# w.2) (# v.2))) →
+      WP App (# w.1) (# v.1) {{ z, ∃ z', j ⤇ (fill K (# z')) ★ τ2i (z, z') }})%I.
+  Next Obligation. 
     intros τ1i τ2i n [x1 x2] [y1 y2] [H1 H2]; simpl in *.
     rewrite H1 H2; trivial.
   Qed.
-  Next Obligation.
-    intros τ1i n τi τi' Hτi z; simpl in *.
-    apply always_ne;
-      apply forall_ne =>j; apply forall_ne =>K; apply forall_ne =>v.
-    apply impl_ne; trivial.
-    apply wp_ne => t; apply exist_ne => h. rewrite Hτi; trivial.
-  Qed.
-  Next Obligation.
-    intros n τi τi' Hτi τ2i z; simpl in *.
-    apply always_ne;
-      apply forall_ne =>j; apply forall_ne =>K; apply forall_ne =>v.
-    apply impl_ne; trivial. rewrite Hτi; trivial.
-  Qed.
+  Next Obligation. solve_proper. Qed.
+  Next Obligation. solve_proper. Qed.
 
   Program Definition interp_forall :
-    ((bivalC -n> iPropG lang Σ) -n> (bivalC -n> iPropG lang Σ)) -n>
-    bivalC -n> iPropG lang Σ :=
-    {|
-      cofe_mor_car :=
-        λ τi,
-        {|
-          cofe_mor_car :=
-            λ w,
-            (∀ (τ'i : {f : (bivalC -n> iPropG lang Σ) |
-                       ∀ vw, PersistentP (f vw)}%type),
-                □ (∀ j K,
-                      j ⤇ (fill K (TApp (# w.2))) →
-                      WP TApp (# w.1) {{v, ∃ v', j ⤇ (fill K (# v')) ★
-                                      (τi (`τ'i) (v, v'))}}))%I
-        |}
-    |}.
+      ((bivalC -n> iPropG lang Σ) -n> (bivalC -n> iPropG lang Σ)) -n>
+      bivalC -n> iPropG lang Σ := λne τi w,
+    (□ ∀ (f : bivalC -n> iPropG lang Σ) j K,
+       (■ (∀ vw, PersistentP (f vw))) →
+       j ⤇ (fill K (TApp (# w.2))) →
+       WP TApp (# w.1) {{ v, ∃ v', j ⤇ fill K (# v') ★ τi f (v, v')}})%I.
   Next Obligation.
     intros τi n [x1 x2] [y1 y2 ] [H1 H2]. simpl in *; auto.
     inversion H1; subst; inversion H2; subst; trivial.
   Qed.
-  Next Obligation.
-    intros n f g Hfg x; cbn.
-    apply forall_ne=> P.
-    apply always_ne.
-    apply forall_ne => j; apply forall_ne => K.
-    apply impl_ne; trivial. apply wp_ne => w; apply exist_ne => v'.
-    rewrite Hfg; trivial.
-  Qed.
+  Next Obligation. solve_proper. Qed.
 
   Program Definition interp_rec_pre :
-    ((bivalC -n> iPropG lang Σ) -n> (bivalC -n> iPropG lang Σ)) -n>
-    (bivalC -n> iPropG lang Σ) -n>
-    (bivalC -n> iPropG lang Σ) :=
-    {|
-      cofe_mor_car :=
-        λ τi,
-        {| cofe_mor_car :=
-             λ rec_appr,
-             {|
-               cofe_mor_car :=
-                 λ w, (□ (∃ v, w = (FoldV (v.1), FoldV (v.2)) ∧
-                               ▷ (τi rec_appr v)))%I
-             |}
-        |}
-    |}.
+      ((bivalC -n> iPropG lang Σ) -n> (bivalC -n> iPropG lang Σ)) -n>
+      (bivalC -n> iPropG lang Σ) -n>
+      (bivalC -n> iPropG lang Σ) := λne τi rec_appr w,
+    (□ (∃ v, w = (FoldV (v.1), FoldV (v.2)) ∧ ▷ (τi rec_appr v)))%I.
   Next Obligation.
     intros τi rec_appr n [x1 x2] [y1 y2] [H1 H2]; simpl in *.
     inversion H1; inversion H2; subst; trivial.
   Qed.
-  Next Obligation.
-    intros τi n f g Hfg x. cbn.
-    apply always_ne, exist_ne =>w; rewrite Hfg; trivial.
-  Qed.
-  Next Obligation.
-    intros n τi τi' Hτi f x. cbn.
-    apply always_ne, exist_ne =>w; rewrite Hτi; trivial.
-  Qed.
+  Next Obligation. solve_proper. Qed.
+  Next Obligation. solve_proper. Qed.
 
   Global Instance interp_rec_pre_contr
-         (τi : (bivalC -n> iPropG lang Σ) -n> (bivalC -n> iPropG lang Σ))
-    :
-      Contractive (interp_rec_pre τi).
+      (τi : (bivalC -n> iPropG lang Σ) -n> (bivalC -n> iPropG lang Σ)) :
+    Contractive (interp_rec_pre τi).
   Proof.
     intros n f g H w; cbn.
     apply always_ne, exist_ne; intros e; apply and_ne; trivial.
-    apply later_contractive =>i Hi.
-    rewrite H; trivial.
+    apply later_contractive =>i Hi. rewrite H; trivial.
   Qed.
 
   Program Definition interp_rec :
-    ((bivalC -n> iPropG lang Σ) -n> (bivalC -n> iPropG lang Σ)) -n>
-    (bivalC -n> iPropG lang Σ)
-    :=
-      {|
-        cofe_mor_car := λ τi, fixpoint (interp_rec_pre τi)
-      |}.
-  Next Obligation.
-  Proof. intros n f g H; apply fixpoint_ne => z; rewrite H; trivial. Qed.
+      ((bivalC -n> iPropG lang Σ) -n> (bivalC -n> iPropG lang Σ)) -n>
+      (bivalC -n> iPropG lang Σ) := λne τi,
+    fixpoint (interp_rec_pre τi).
+  Next Obligation. intros n f g H; apply fixpoint_ne => z; rewrite H; trivial. Qed.
 
   Context `{i : heapIG Σ} (L : namespace).
 
   Program Definition interp_ref_pred (l : loc * loc) :
-    (bivalC -n> iPropG lang Σ) -n> iPropG lang Σ :=
-    {|
-      cofe_mor_car := λ τi, (∃ v, (l.1) ↦ᵢ (v.1) ★ (l.2) ↦ₛ (v.2) ★ (τi v))%I
-    |}.
-  Next Obligation.
-  Proof. intros ???? H; apply exist_ne =>w; rewrite H; trivial. Qed.
+      (bivalC -n> iPropG lang Σ) -n> iPropG lang Σ := λne τi,
+    (∃ v, (l.1) ↦ᵢ (v.1) ★ (l.2) ↦ₛ (v.2) ★ (τi v))%I.
+  Next Obligation. solve_proper. Qed.
 
   Program Definition interp_ref :
-    (bivalC -n> iPropG lang Σ) -n> bivalC -n> iPropG lang Σ :=
-    {|
-      cofe_mor_car :=
-        λ τi, {|
-          cofe_mor_car :=
-            λ w, (∃ l, w = (LocV (l.1), LocV (l.2)) ∧
-                       inv (L .@ l) (interp_ref_pred l τi))%I
-        |}
-    |}.
+      (bivalC -n> iPropG lang Σ) -n> bivalC -n> iPropG lang Σ := λne τi w,
+    (∃ l, w = (LocV (l.1), LocV (l.2)) ∧ inv (L .@ l) (interp_ref_pred l τi))%I.
   Next Obligation.
     intros τi n [x1 x2] [y1 y2] [H1 H2]; simpl in *.
     inversion H1; inversion H2; subst; trivial.
   Qed.
-  Next Obligation.
-    intros n τi τi' Hτi z; simpl in *.
-    apply exist_ne=>w; apply and_ne; trivial; cbn.
-    apply (contractive_ne _); apply exist_ne=>w'; rewrite Hτi; trivial.
-  Qed.
+  Next Obligation. solve_proper. Qed.
 
-  Program Fixpoint interp (τ : type) {struct τ}
-    : (varC -n> bivalC -n> iPropG lang Σ) -n> bivalC -n> iPropG lang Σ
-    :=
-      match τ return (varC -n> bivalC -n> iPropG lang Σ) -n>
-                     bivalC -n> iPropG lang Σ
-      with
-      | TUnit => {| cofe_mor_car := λ Δ, interp_unit |}
-      | TNat => {| cofe_mor_car := λ Δ, interp_nat |}
-      | TBool => {| cofe_mor_car := λ Δ, interp_bool |}
-      | TProd τ1 τ2 =>
-        {| cofe_mor_car := λ Δ, interp_prod (interp τ1 Δ) (interp τ2 Δ)|}
-      | TSum τ1 τ2 =>
-        {| cofe_mor_car := λ Δ, interp_sum(interp τ1 Δ) (interp τ2 Δ)|}
-      | TArrow τ1 τ2 =>
-        {|cofe_mor_car := λ Δ, interp_arrow (interp τ1 Δ) (interp τ2 Δ)|}
-      | TVar v => {| cofe_mor_car := λ Δ, (Δ v)  |}
-      | TForall τ' =>
-        {| cofe_mor_car :=
-             λ Δ, interp_forall  (extend_context_interp_apply Δ (interp τ')) |}
-      | TRec τ' =>
-        {| cofe_mor_car :=
-             λ Δ, interp_rec
-                    (extend_context_interp_apply Δ (interp τ')) |}
-      | Tref τ' => {| cofe_mor_car := λ Δ, interp_ref (interp τ' Δ) |}
-      end%I.
+  Program Fixpoint interp (τ : type) {struct τ} :
+      (varC -n> bivalC -n> iPropG lang Σ) -n> bivalC -n> iPropG lang Σ :=
+    match τ return (varC -n> bivalC -n> iPropG lang Σ) -n>
+                   bivalC -n> iPropG lang Σ with
+    | TUnit => λne Δ, interp_unit
+    | TNat => λne Δ, interp_nat
+    | TBool => λne Δ, interp_bool
+    | TProd τ1 τ2 => λne Δ, interp_prod (interp τ1 Δ) (interp τ2 Δ)
+    | TSum τ1 τ2 => λne Δ, interp_sum(interp τ1 Δ) (interp τ2 Δ)
+    | TArrow τ1 τ2 => λne Δ, interp_arrow (interp τ1 Δ) (interp τ2 Δ)
+    | TVar v => λne Δ, (Δ v)
+    | TForall τ' =>λne Δ, interp_forall  (extend_context_interp_apply Δ (interp τ'))
+    | TRec τ' => λne Δ, interp_rec (extend_context_interp_apply Δ (interp τ'))
+    | Tref τ' => λne Δ, interp_ref (interp τ' Δ)
+    end%I.
   Solve Obligations
   with repeat intros ?;
               match goal with [H : _ ≡{_}≡ _|- _] => rewrite H end; trivial.
 
   Global Instance interp_Persistent
-         τ (Δ : varC -n> bivalC -n> iPropG lang Σ)
-         {HΔ : ∀ x vw, PersistentP (Δ x vw)}
-    : ∀ vw, PersistentP (interp τ Δ vw).
+      τ (Δ : varC -n> bivalC -n> iPropG lang Σ)
+      {HΔ : ∀ x vw, PersistentP (Δ x vw)} :
+    ∀ vw, PersistentP (interp τ Δ vw).
   Proof.
     revert Δ HΔ.
     induction τ; cbn; intros Δ HΔ v; try apply _.
@@ -426,27 +267,21 @@ Section logrel.
   Qed.
 
   Program Definition hop_context_interp (m n : nat) :
-    (varC -n> bivalC -n> iPropG lang Σ) -n>
-    (varC -n> bivalC -n> iPropG lang Σ) :=
-    {| cofe_mor_car :=
-         λ Δ,
-         {| cofe_mor_car := λ v, if lt_dec v m then Δ v else Δ (v - n) |}
-    |}.
-  Next Obligation.
-  Proof. intros ?????? Hxy; destruct Hxy; trivial. Qed.
+      (varC -n> bivalC -n> iPropG lang Σ) -n>
+      (varC -n> bivalC -n> iPropG lang Σ) := λne Δ v,
+    if lt_dec v m then Δ v else Δ (v - n).
+  Next Obligation. intros ?????? Hxy; destruct Hxy; trivial. Qed.
   Next Obligation.
     intros ????? Hfg ?; cbn. destruct lt_dec; rewrite Hfg; trivial.
   Qed.
 
   Lemma extend_bofore_hop_context_interp (m n : nat)
-        (Δ : varC -n> bivalC -n> iPropG lang Σ)
-        (τi : bivalC -n> iPropG lang Σ)
-        (v : var)
-    :
-      (extend_context_interp τi (hop_context_interp m n Δ)
-                             (if lt_dec v (S m) then v else n + v))
-        ≡ (hop_context_interp (S m) n (extend_context_interp τi Δ)
-                              (if lt_dec v (S m) then v else n + v)).
+      (Δ : varC -n> bivalC -n> iPropG lang Σ)
+      (τi : bivalC -n> iPropG lang Σ) (v : var) :
+    extend_context_interp τi (hop_context_interp m n Δ)
+                             (if lt_dec v (S m) then v else n + v)
+    ≡ hop_context_interp (S m) n (extend_context_interp τi Δ)
+                                 (if lt_dec v (S m) then v else n + v).
   Proof.
     destruct v; cbn; trivial.
     repeat (destruct lt_dec; cbn); auto with omega.
@@ -459,10 +294,8 @@ Section logrel.
   Qed.
 
   Lemma interp_subst_weaken
-        (m n : nat)
-        (Δ : varC -n> bivalC -n> iPropG lang Σ)
-        (τ : type)
-    : interp τ Δ ≡ interp τ.[iter m up (ren (+n))] (hop_context_interp m n Δ).
+      (m n : nat) (Δ : varC -n> bivalC -n> iPropG lang Σ) (τ : type) :
+    interp τ Δ ≡ interp τ.[iter m up (ren (+n))] (hop_context_interp m n Δ).
   Proof.
     revert m n Δ.
     induction τ; intros m n Δ v; cbn -[extend_context_interp]; auto.
@@ -483,12 +316,7 @@ Section logrel.
       asimpl; unfold ids; cbn; destruct lt_dec; cbn; destruct lt_dec; auto with omega.
       replace (m + n + (x - m)) with (x + n) by omega.
       replace (x + n - n) with x; trivial.
-      { (** An incompleteness in omega and lia! *)
-        clear.
-        replace (x + n) with (n + x) by omega.
-        induction n; cbn; auto with omega.
-        induction x; cbn; trivial.
-      }
+      { unfold var in *; omega. }
     - properness; trivial.
       change (up (iter m up (ren (+n)))) with (iter (S m) up (ren (+n))).
       rewrite IHτ.
@@ -498,51 +326,37 @@ Section logrel.
   Qed.
 
   Lemma interp_ren_S (τ : type)
-        (Δ : varC -n> bivalC -n> iPropG lang Σ)
-        (τi : bivalC -n> iPropG lang Σ)
-    : interp τ Δ ≡ interp τ.[ren (+1)] (extend_context_interp τi Δ).
+      (Δ : varC -n> bivalC -n> iPropG lang Σ) (τi : bivalC -n> iPropG lang Σ) :
+    interp τ Δ ≡ interp τ.[ren (+1)] (extend_context_interp τi Δ).
   Proof.
     rewrite (interp_subst_weaken 0 1).
     apply interp_unused_contex_irrel.
-    { clear. intros [|v]; cbn; trivial. }
+    clear. intros [|v]; cbn; trivial.
   Qed.
 
   Local Opaque eq_nat_dec.
 
   Program Definition context_interp_insert (m : nat) :
-    (bivalC -n> iPropG lang Σ) -n>
-    (varC -n> bivalC -n> iPropG lang Σ) -n>
-    (varC -n> bivalC -n> iPropG lang Σ) :=
-    {| cofe_mor_car :=
-         λ τi,
-         {| cofe_mor_car :=
-              λ Δ,
-              {| cofe_mor_car :=
-                   λ v, if lt_dec v m then Δ v else
-                          if eq_nat_dec v m then τi else Δ (v - 1)
-              |}
-         |}
-    |}.
+      (bivalC -n> iPropG lang Σ) -n>
+      (varC -n> bivalC -n> iPropG lang Σ) -n>
+      (varC -n> bivalC -n> iPropG lang Σ) := λne τi Δ v,
+    if lt_dec v m then Δ v else if eq_nat_dec v m then τi else Δ (v - 1).
+  Next Obligation. intros m τi Δ n x y Hxy; destruct Hxy; trivial. Qed.
   Next Obligation.
-  Proof. intros m τi Δ n x y Hxy; destruct Hxy; trivial. Qed.
-  Next Obligation.
-  Proof.
     intros m τi n Δ Δ' HΔ x; cbn;
       destruct lt_dec; try destruct eq_nat_dec; auto.
   Qed.
   Next Obligation.
-  Proof.
     intros m n f g Hfg F Δ x; cbn;
       destruct lt_dec; try destruct eq_nat_dec; auto.
   Qed.
 
   Lemma extend_context_interp_insert (m : nat)
-        (τi : bivalC -n> iPropG lang Σ)
-        (Δ : varC -n> bivalC -n> iPropG lang Σ)
-        (Ti : bivalC -n> iPropG lang Σ)
-    :
-      (extend_context_interp Ti (context_interp_insert m τi Δ))
-        ≡ (context_interp_insert (S m) τi (extend_context_interp Ti Δ)).
+      (τi : bivalC -n> iPropG lang Σ)
+      (Δ : varC -n> bivalC -n> iPropG lang Σ)
+      (Ti : bivalC -n> iPropG lang Σ) :
+    extend_context_interp Ti (context_interp_insert m τi Δ)
+    ≡ context_interp_insert (S m) τi (extend_context_interp Ti Δ).
   Proof.
     intros [|v]; cbn; trivial.
     repeat destruct lt_dec; trivial;
@@ -552,11 +366,9 @@ Section logrel.
   Qed.
 
   Lemma context_interp_insert_O_extend
-        (τi : bivalC -n> iPropG lang Σ)
-        (Δ : varC -n> bivalC -n> iPropG lang Σ)
-    :
-      (context_interp_insert O τi Δ)
-        ≡ (extend_context_interp τi Δ).
+      (τi : bivalC -n> iPropG lang Σ)
+      (Δ : varC -n> bivalC -n> iPropG lang Σ) :
+    context_interp_insert O τi Δ ≡ extend_context_interp τi Δ.
   Proof.
     intros [|v]; cbn; trivial.
     repeat destruct lt_dec; trivial;
@@ -565,7 +377,7 @@ Section logrel.
   Qed.
 
   Lemma iter_up_subst_type (m : nat) (τ : type) (x : var) :
-      (iter m up (τ .: ids) x) =
+    iter m up (τ .: ids) x =
       if lt_dec x m then ids x else
         if eq_nat_dec x m then τ.[ren (+m)] else ids (x - 1).
   Proof.
@@ -582,12 +394,9 @@ Section logrel.
   Qed.
 
   Lemma interp_subst_iter_up
-        (m : nat)
-        (Δ : varC -n> bivalC -n> iPropG lang Σ)
-        (τ : type)
-        (τ' : type)
-    : interp τ (context_interp_insert m (interp τ'.[ren (+m)] Δ) Δ)
-             ≡ interp τ.[iter m up (τ' .: ids)] Δ.
+      (m : nat) (Δ : varC -n> bivalC -n> iPropG lang Σ) (τ τ' : type) :
+    interp τ (context_interp_insert m (interp τ'.[ren (+m)] Δ) Δ)
+    ≡ interp τ.[iter m up (τ' .: ids)] Δ.
   Proof.
     revert m Δ.
     induction τ; intros m Δ v; cbn -[extend_context_interp]; auto.
@@ -620,10 +429,8 @@ Section logrel.
   Qed.
 
   Lemma interp_subst
-        (Δ : varC -n> bivalC -n> iPropG lang Σ)
-        (τ : type)
-        (τ' : type)
-    : interp τ (extend_context_interp (interp τ' Δ) Δ) ≡ interp τ.[τ'/] Δ.
+      (Δ : varC -n> bivalC -n> iPropG lang Σ) (τ τ' : type) :
+    interp τ (extend_context_interp (interp τ' Δ) Δ) ≡ interp τ.[τ'/] Δ.
   Proof.
     rewrite -(interp_subst_iter_up O Δ τ τ').
     rewrite context_interp_insert_O_extend.
@@ -631,22 +438,20 @@ Section logrel.
   Qed.
 
   Lemma zip_with_context_interp_subst
-        (Δ : varC -n> bivalC -n> iPropG lang Σ) (Γ : list type)
-        (vs : list bivalC) (τi : bivalC -n> iPropG lang Σ) :
-    ([∧] zip_with (λ τ, interp τ Δ) Γ vs)%I
-      ≡ ([∧] zip_with (λ τ, interp τ (extend_context_interp τi Δ))
-                    (map (λ t : type, t.[ren (+1)]) Γ) vs)%I.
+      (Δ : varC -n> bivalC -n> iPropG lang Σ) (Γ : list type)
+      (vs : list bivalC) (τi : bivalC -n> iPropG lang Σ) :
+    ([∧] zip_with (λ τ, interp τ Δ) Γ vs)
+    ⊣⊢ ([∧] zip_with (λ τ, interp τ (extend_context_interp τi Δ))
+                     (map (λ t : type, t.[ren (+1)]) Γ) vs).
   Proof.
     revert Δ vs τi.
     induction Γ as [|Γ]; intros Δ vs τi; cbn; trivial.
     destruct vs; cbn; trivial.
-    apply and_proper.
-    - apply interp_ren_S.
-    - apply IHΓ.
+    apply and_proper. apply interp_ren_S. apply IHΓ.
   Qed.
 
   Lemma EqType_related_eq τ {H : EqType τ} v v' (Δ : varC -n> bivalC -n> iPropG lang Σ)
-        {HΔ : ∀ x vw, PersistentP (Δ x vw)} :
+      {HΔ : ∀ x vw, PersistentP (Δ x vw)} :
     interp τ Δ (v, v') ⊢ ■ (v = v').
   Proof.
     revert v v'; induction H => v v'; iIntros "#H1".
